proofs/x86-64/avx2/ml_dsa_65/polynomial.ec
@@ -19,27 +19,40 @@ op check_inf_norm_circuit (_a : W32.t Array256.t) (_threshold : int) : bool =
 
 lemma polynomial____check_infinity_norm_correct (_a : W32.t Array256.t) (_threshold : int) :
    hoare [ M.polynomial____check_infinity_norm :
-       _threshold = (1 `<<` gamma1m1_bits) - 49 * w1_bits /\
+       (* gamma1-Beta = 524092  or  gamma2-Beta = 261692 *)
+       (_threshold = (1 `<<` gamma1m1_bits) - 49 * w1_bits \/
+        _threshold = (q - 1) %/ 32 - 49 * w1_bits) /\
        polynomial = _a /\ threshold = _threshold /\
-       wpoly_srng (gamma1-1) gamma1 _a
+       (* coefficients must be centered representatives so to_sint = crepr *)
+       wpoly_srng ((q-1) %/ 2) ((q-1) %/ 2) _a
      ==>
        (wpoly_infnorm_lt _threshold _a => res = W64.zero) /\
-       (!wpoly_infnorm_lt _threshold _a => res <> W64.zero)
+       (!wpoly_infnorm_lt _threshold _a => res = W64.one)
    ].
 proof.
 rewrite /(`<<`) /=.
 proc => /=.
-seq 2 : (#pre /\ threshold_vector = W256.of_int (524091)).
-+ auto => /> *; rewrite /VMOV_64 /= to_uint_eq to_uint_zeroextu256 of_uintK /=.
-  rewrite -(W128.of_uintK 524091); congr; rewrite wordP => i ib.
-  rewrite /pack2_t initiE 1:/# /= get_of_list 1:/# /= of_intE /= bits2wE initiE 1:/# /=.
-  case (i %/ 64 = 0) => ? /=.
-  + rewrite of_intE /= bits2wE initiE 1:/# /=.
-    by rewrite /BitEncoding.BS2Int.int2bs nth_mkseq 1:/# /= nth_mkseq 1:/# /= /#.
-  rewrite /BitEncoding.BS2Int.int2bs nth_mkseq 1:/# /=.
-  rewrite pdiv_small; last by smt().
-  smt(StdOrder.IntOrder.ler_lt_trans StdOrder.IntOrder.ler_weexpn2l pow2_64).
-  
+seq 2 : (#pre /\ threshold_vector = W256.of_int (_threshold - 1)).
++ auto => />  Hdisj; elim Hdisj => [-> | ->] /= Hrng.
+  + rewrite /VMOV_64 /= to_uint_eq to_uint_zeroextu256 of_uintK /=.
+    rewrite -(W128.of_uintK 524091); congr; rewrite wordP => i ib.
+    rewrite /pack2_t initiE 1:/# /= get_of_list 1:/# /= of_intE /= bits2wE initiE 1:/# /=.
+    case (i %/ 64 = 0) => ? /=.
+    + rewrite of_intE /= bits2wE initiE 1:/# /=.
+      by rewrite /BitEncoding.BS2Int.int2bs nth_mkseq 1:/# /= nth_mkseq 1:/# /= /#.
+    rewrite /BitEncoding.BS2Int.int2bs nth_mkseq 1:/# /=.
+    rewrite pdiv_small; last by smt().
+    smt(StdOrder.IntOrder.ler_lt_trans StdOrder.IntOrder.ler_weexpn2l pow2_64).
+  + rewrite /VMOV_64 /= to_uint_eq to_uint_zeroextu256 of_uintK /=.
+    rewrite -(W128.of_uintK 261691); congr; rewrite wordP => i ib.
+    rewrite /pack2_t initiE 1:/# /= get_of_list 1:/# /= of_intE /= bits2wE initiE 1:/# /=.
+    case (i %/ 64 = 0) => ? /=.
+    + rewrite of_intE /= bits2wE initiE 1:/# /=.
+      by rewrite /BitEncoding.BS2Int.int2bs nth_mkseq 1:/# /= nth_mkseq 1:/# /= /#.
+    rewrite /BitEncoding.BS2Int.int2bs nth_mkseq 1:/# /=.
+    rewrite pdiv_small; last by smt().
+    smt(StdOrder.IntOrder.ler_lt_trans StdOrder.IntOrder.ler_weexpn2l pow2_64).
+
 proc change ^while.1 : { coefficients <- if (0 <= offset*8 <= 32*256-256)
                                          then BSWAS_256u32_256.sliceget polynomial (offset*8)
                                          else get256_direct (WArray1024.init32 (fun i => polynomial.[i])) offset; }.
@@ -50,31 +63,46 @@ proc change ^while.1 : { coefficients <- if (0 <= offset*8 <= 32*256-256)
 wp 7.
 proc change 7 : { zf <- msb_mask = W32.zero; }.
 + by auto => /= &1 &2 ->; rewrite /TEST_32 /rflags_of_bwop /= /ZF_of  /=.
-                  
+
 unroll for ^while.
 cfold 131.
 wp -1.
-conseq (: polynomial = _a /\ threshold_vector = W256.of_int 524091 /\
-          all (fun i => W32.of_int (-(524288-1)) \sle _a.[i] /\ _a.[i] \sle W32.of_int 524288) (iotared 0 256) ==>
-    zf =  (check_inf_norm_circuit _a 524092)); last 
-     by rewrite  /check_inf_norm_circuit /=; circuit.  
-
+conseq (: polynomial = _a /\ threshold_vector = W256.of_int (_threshold - 1) /\
+        List.all (fun i => W32.of_int (-4190208) \sle _a.[i]
+               /\ _a.[i] \sle  W32.of_int 4190208) (iotared 0 256) /\
+          (_threshold = 524092 \/ _threshold = 261692)  ==>
+    zf = (check_inf_norm_circuit _a _threshold)). 
 
 (*  Connect circuit form to poly_infnorm spec *)
-+ move =>  &1; rewrite iotaredE mldsa65_gamma1 => |>; rewrite /wpoly_srng !allP /= => H.
-  move => x; rewrite mem_iota /= => *; rewrite /(\sle) /= !of_sintK /= /smod /= /#.
++ move => &1 [#] ? <- ? + ?; rewrite /wpoly_srng iotaredE /(\sle) !of_sintK /smod !allP /=;smt(mem_iota).
 
-move => &hr [[H H1] H2] msbm -> /=; rewrite /wpoly_infnorm /wpoly_srng /check_inf_norm_circuit !allP /SETcc;split;rewrite iotaredE /TEST_32 /= => H3.
+move => &hr [#] Hdij <- Ht Hr ? zf  -> /=.
+rewrite /wpoly_infnorm /wpoly_srng /check_inf_norm_circuit !allP /SETcc;
+split; rewrite iotaredE /TEST_32 /= => H4.
 + rewrite ifF /=.
-  + rewrite  /(\slt) /= !of_sintK /= /smod /=.
+  + rewrite /(\slt) /= !of_sintK /= /smod /=.
     move => x; rewrite mem_iota => ?.
-    move : H3; rewrite /wpoly_infnorm_lt /wpoly_srng allP /= /#.
+    move : H4; rewrite /wpoly_infnorm_lt /wpoly_srng allP /= /#.
   by rewrite to_uint_eq /=.
-    
 rewrite ifT /=.
-  + rewrite  /(\slt) /= !of_sintK /= /smod /=.
-    move : H3; rewrite /wpoly_infnorm_lt /wpoly_srng allP /=;smt(mem_iota).
+  + rewrite /(\slt) /= !of_sintK /= /smod /=.
+    move : H4; rewrite /wpoly_infnorm_lt /wpoly_srng allP /=; smt(mem_iota).
   by rewrite to_uint_eq /=.
+
+  (* Handle the circuit *)
+case (_threshold = 524092).
++ conseq (: polynomial = _a /\ threshold_vector = W256.of_int 524091 /\
+       List.all (fun i => W32.of_int (-4190208) \sle _a.[i]
+               /\ _a.[i] \sle  W32.of_int 4190208) (iotared 0 256)
+          ==>
+    zf = (check_inf_norm_circuit _a 524092));
+    [ by smt() | by smt() | by simplify;circuit]. 
++ conseq (: polynomial = _a /\ threshold_vector = W256.of_int 261691 /\
+       List.all (fun i => W32.of_int (-4190208) \sle _a.[i]
+               /\ _a.[i] \sle  W32.of_int 4190208) (iotared 0 256)
+          ==>
+    zf = (check_inf_norm_circuit _a 261692));
+    [ by smt() | by smt() | by simplify;circuit]. 
 qed.
 
 lemma polynomial____check_infinity_norm_ll : islossless M.polynomial____check_infinity_norm.
@@ -85,11 +113,14 @@ qed.
 
 lemma polynomial____check_infinity_norm_ph (_a : W32.t Array256.t) (_threshold : int) :
    phoare [ M.polynomial____check_infinity_norm :
-       _threshold = (1 `<<` gamma1m1_bits) - 49 * w1_bits /\
+       (* gamma1-Beta = 524092  or  gamma2-Beta = 261692 *)
+       (_threshold = (1 `<<` gamma1m1_bits) - 49 * w1_bits \/
+        _threshold = (q - 1) %/ 32 - 49 * w1_bits) /\
        polynomial = _a /\ threshold = _threshold /\
-       wpoly_srng (gamma1-1) gamma1 _a
+       (* coefficients must be centered representatives so to_sint = crepr *)
+       wpoly_srng ((q-1) %/ 2) ((q-1) %/ 2) _a
      ==>
        (wpoly_infnorm_lt _threshold _a => res = W64.zero) /\
-       (!wpoly_infnorm_lt _threshold _a => res <> W64.zero)
+       (!wpoly_infnorm_lt _threshold _a => res = W64.one)
    ] = 1%r
- by  conseq polynomial____check_infinity_norm_ll (polynomial____check_infinity_norm_correct _a _threshold).
+ by conseq polynomial____check_infinity_norm_ll (polynomial____check_infinity_norm_correct _a _threshold).
